fix to examples

compiler/src/compilerExamples/immediateExample.v
@@ -56,11 +56,16 @@ Notation RiscvMachine := MetricRiscvMachine.
 Local Existing Instance coqutil.Map.SortedListString.map.
 Local Existing Instance coqutil.Map.SortedListString.ok.
 
-Definition main_stackalloc :=
+Definition main_stackalloc : (string * (list string * list string * cmd)) :=
   ("main", ([]: list String.string, []: list String.string,
-     cmd.stackalloc "x" 4 (cmd.stackalloc "y" 4 (cmd.call [] "swap_swap" [expr.var "x"; expr.var "y"])))).
+                 cmd.stackalloc "x" 4 (cmd.stackalloc "y" 4 (cmd.call [] "imm_ex" [expr.var "x"; expr.var "y"])))).
 
-Definition allFuns: list Syntax.func := [swap; swap_swap; main_stackalloc; stacknondet; stackdisj; long1].
+
+Definition immediate_example : (string * (list string * list string * cmd )) :=
+  ("imm_ex", ([]: list String.string, ["a"; "b"],
+                 cmd.seq (cmd.set "a" (expr.op bopname.sub (expr.literal 38) (expr.literal 31))) (cmd.set "b" (expr.op bopname.and (expr.var "a") (expr.literal 16))))).
+
+Definition allFuns: list (string * (list string * list string * cmd)) := [immediate_example; main_stackalloc].
 
 (* stack grows from high addreses to low addresses, first stack word will be written to
    (stack_pastend-8), next stack word to (stack_pastend-16) etc *)
@@ -82,7 +87,7 @@ Proof. intros. congruence. Qed.
 Local Instance RV32I_bitwidth: FlatToRiscvCommon.bitwidth_iset 32 RV32I.
 Proof. reflexivity. Qed.
 
-Definition swap_asm: list Instruction.
+Definition imm_asm: list Instruction.
   let r := eval cbv in (compile compile_ext_call allFuns) in set (res := r).
   match goal with
   | res := Success (?x, _, _) |- _ => exact x
@@ -91,126 +96,14 @@ Defined.
 
 Module PrintAssembly.
   Import riscv.Utility.InstructionNotations.
-  Goal True. let r := eval unfold swap_asm in swap_asm in idtac (* r *). Abort.
-  (*
-  swap_swap:
-     addi    x2, x2, -20   // decrease sp
-     sw      x2, x1, 8     // save ra
-     sw      x2, x3, 0     // save registers modified by swap_swap
-     sw      x2, x4, 4
-     lw      x3, x2, 12    // load args
-     lw      x4, x2, 16
-     sw      x2, x3, -8    // store args for first call to swap
-     sw      x2, x4, -4
-     jal     x1, 36        // first call to swap
-     sw      x2, x3, -8    // store args for second call to swap
-     sw      x2, x4, -4
-     jal     x1, 24        // second call to swap
-     lw      x3, x2, 0     // restore registers modified by swap_swap
-     lw      x4, x2, 4
-     lw      x1, x2, 8     // load ra
-     addi    x2, x2, 20    // increase sp
-     jalr    x0, x1, 0     // return
-
-  swap:
-     addi    x2, x2, -28   // decrease sp
-     sw      x2, x1, 16    // save ra
-     sw      x2, x5, 0     // save registers modified by swap
-     sw      x2, x6, 4
-     sw      x2, x3, 8
-     sw      x2, x4, 12
-     lw      x3, x2, 20    // load args
-     lw      x4, x2, 24
-     lw      x5, x4, 0     // body of swap
-     lw      x6, x3, 0
-     sw      x4, x6, 0
-     sw      x3, x5, 0
-     lw      x5, x2, 0     // restore registers modified by swap
-     lw      x6, x2, 4
-     lw      x3, x2, 8
-     lw      x4, x2, 12
-     lw      x1, x2, 16    // restore ra
-     addi    x2, x2, 28    // increase sp
-     jalr    x0, x1, 0     // return
-
-  stacknondet:
-     addi    x2, x2, -56
-     sw      x2, x1, 44
-     sw      x2, x5, 4
-     sw      x2, x6, 8
-     sw      x2, x7, 12
-     sw      x2, x3, 16
-     sw      x2, x8, 20
-     sw      x2, x9, 24
-     sw      x2, x10, 28
-     sw      x2, x11, 32
-     sw      x2, x12, 36
-     sw      x2, x4, 40
-     addi    x5, x2, 0
-     lw      x6, x5, 0
-     addi    x7, x0, 8
-     srl     x3, x6, x7
-     addi    x8, x0, 3
-     add     x9, x3, x8
-     addi    x10, x0, 42
-     sb      x9, x10, 0
-     lw      x11, x5, 0
-     addi    x12, x0, 8
-     srl     x4, x11, x12
-     sw      x2, x3, 48
-     sw      x2, x4, 52
-     lw      x5, x2, 4
-     lw      x6, x2, 8
-     lw      x7, x2, 12
-     lw      x3, x2, 16
-     lw      x8, x2, 20
-     lw      x9, x2, 24
-     lw      x10, x2, 28
-     lw      x11, x2, 32
-     lw      x12, x2, 36
-     lw      x4, x2, 40
-     lw      x1, x2, 44
-     addi    x2, x2, 56
-     jalr    x0, x1, 0
-
-  stackdisj:
-     addi    x2, x2, -28
-     sw      x2, x1, 16
-     sw      x2, x3, 8
-     sw      x2, x4, 12
-     addi    x3, x2, 4
-     addi    x4, x2, 0
-     sw      x2, x3, 20
-     sw      x2, x4, 24
-     lw      x3, x2, 8
-     lw      x4, x2, 12
-     lw      x1, x2, 16
-     addi    x2, x2, 28
-     jalr    x0, x1, 0
-
-  main:
-     addi    x2, x2, -20   // decrease sp
-     sw      x2, x1, 16    // save ra
-     sw      x2, x3, 8     // save registers modified by main
-     sw      x2, x4, 12
-     addi    x3, x2, 4     // first stackalloc invocation returns sp+4
-     addi    x4, x2, 0     // second stackalloc invocation returns sp
-     sw      x2, x3, -8    // store args for call to swap_swap
-     sw      x2, x4, -4
-     jal     x1, -380      // call swap_swap
-     lw      x3, x2, 8     // restore registers modified by main
-     lw      x4, x2, 12
-     lw      x1, x2, 16    // restore ra
-     addi    x2, x2, 20    // increase sp
-     jalr    x0, x1, 0     // return
-  *)
+  Goal True. let r := eval unfold imm_asm in imm_asm in idtac (* r *). Abort.
 End PrintAssembly.
 
-Definition swap_as_bytes: list Byte.byte := instrencode swap_asm.
+Definition imm_as_bytes: list Byte.byte := instrencode imm_asm.
 
 Module PrintBytes.
   Import bedrock2.Hexdump.
   Local Open Scope hexdump_scope.
   Set Printing Width 100.
-  Goal True. let x := eval cbv in swap_as_bytes in idtac (* x *). Abort.
+  Goal True. let x := eval cbv in imm_as_bytes in idtac (* x *). Abort.
 End PrintBytes.
